correct matching on unk and err

cast-tests/castcic.v
@@ -1,18 +1,16 @@
 From MetaCoq.Template Require Import TemplateMonad config utils Loader.
 From MetaCoq.PCUIC Require Import PCUICAst PCUICToTemplate PCUICPretty PCUICSN PCUICTyping PCUICNormal.
 From MetaCoq.SafeChecker Require Import PCUICErrors SafeTemplateChecker PCUICWfEnvImpl PCUICWfEnv PCUICSafeChecker PCUICSafeReduce.
+From Coq Require Import Nat.
 Import MCMonadNotation.
 
 Global Existing Instance PCUICSN.default_normalizing.
 
-Check typecheck_program.
-Check PCUICSafeReduce.hnf.
-Check check_wf_type.
-
-Axiom unk : forall (A : Type), A.
+Axiom castcic_unk : forall (A : Type), A.
 Axiom castcic_err : forall (A : Type), A.
 Axiom castcic_cast : forall (A B : Type), A -> B.
 
+Notation unk := castcic_unk.
 Notation err := castcic_err.
 Notation cast := castcic_cast.
 
@@ -27,7 +25,32 @@ Program Definition eval_compute_cheat (cf := default_checker_flags)
     [] p'.2 (todo "welltyped") in
     PCUICToTemplate.trans tm.
 
-MetaCoq Quote Recursively Definition foo := (1 + pred (1 + (unk nat))).
+Program Definition add0 (n : nat) :=
+  match n return n + 0 = n with
+  | 0 => _
+  | S m => _
+  end.
+Next Obligation.
+todo "".
+Defined.
+MetaCoq Quote Definition bar := Eval lazy in add0.
+Print bar.
+
+Definition even (n : nat) :=
+  match n with
+  | 0 => true
+  | S m => false
+  end.
+
+MetaCoq Quote Definition foo := Eval lazy in (even (unk nat)).
+Print foo.
+Definition pd :=
+  match foo with
+  | tCase _ p _ _ => p
+  | _ => mk_predicate [] [] [] foo
+  end.
 Definition foo' := Eval lazy in eval_compute_cheat foo Monomorphic_ctx.
+Print foo'.
+Definition a := inst_case_predicate_context
 MetaCoq Unquote Definition foo'' := foo'.
 Print foo''.
